Beta.v
@@ -18,3 +18,722 @@ Inductive beta : term -> term -> Prop :=
 | beta_switch1 : forall t1 t2 l, beta t1 t2 -> beta (switch t1 l) (switch t2 l)
 | beta_switch2 : forall t p t1 t2 l1 l2, beta t1 t2 -> beta (switch t (l1 ++ (p, t1) :: l2)) (switch t (l1 ++ (p, t2) :: l2))
 | beta_switch_redex : forall l t l1 l2, beta (switch (constr (length l1) l) (l1 ++ (length l, t) :: l2)) (subst (read_env l) t).
+
+Lemma star_beta_app :
+  forall t1 t2 t3 t4, star beta t1 t2 -> star beta t3 t4 -> star beta (app t1 t3) (app t2 t4).
+Proof.
+  intros t1 t2 t3 t4 H12 H34.
+  eapply star_compose.
+  + eapply star_map_impl with (RA := beta) (f := fun t => app t _); [|eassumption].
+    intros; constructor; assumption.
+  + eapply star_map_impl with (RA := beta) (f := fun t => app _ t); [|eassumption].
+    intros; constructor; assumption.
+Qed.
+
+Lemma star_beta_abs :
+  forall t1 t2, star beta t1 t2 -> star beta (abs t1) (abs t2).
+Proof.
+  intros t1 t2 H12.
+  eapply star_map_impl with (RA := beta) (f := fun t => abs t); [|eassumption].
+  intros; constructor; assumption.
+Qed.
+
+Lemma star_beta_constr :
+  forall tag l1 l2, Forall2 (star beta) l1 l2 -> star beta (constr tag l1) (constr tag l2).
+Proof.
+  intros tag l1 l2 H12.
+  enough (H : forall l, star beta (constr tag (l ++ l1)) (constr tag (l ++ l2))).
+  { exact (H nil). }
+  induction H12 as [|t1 t2 l1 l2 Ht Hl IH].
+  - intros. apply star_refl.
+  - intros l. eapply star_compose.
+    + specialize (IH (l ++ (t1 :: nil))). rewrite <- !app_assoc in IH. simpl in IH. apply IH.
+    + eapply star_map_impl with (RA := beta) (f := fun t => constr tag (l ++ t :: l2)); [|eassumption].
+      intros; constructor; assumption.
+Qed.
+
+Lemma star_beta_switch :
+  forall t1 t2 l1 l2,
+    star beta t1 t2 -> Forall2 (fun pt1 pt2 => fst pt1 = fst pt2 /\ star beta (snd pt1) (snd pt2)) l1 l2 ->
+    star beta (switch t1 l1) (switch t2 l2).
+Proof.
+  intros t1 t2 l1 l2 Ht Hl.
+  eapply star_compose.
+  { eapply star_map_impl with (RA := beta) (f := fun t => switch t _); [|eassumption]; intros; constructor; assumption. }
+  enough (H : forall l, star beta (switch t2 (l ++ l1)) (switch t2 (l ++ l2))).
+  { exact (H nil). }
+  induction Hl as [|pt1 pt2 l1 l2 [Hp H] Hl IH].
+  - intros. apply star_refl.
+  - intros l. eapply star_compose.
+    + specialize (IH (l ++ (pt1 :: nil))). rewrite <- !app_assoc in IH. simpl in IH. apply IH.
+    + destruct pt1 as [p1 t3]; destruct pt2 as [p2 t4]; simpl in *; subst.
+      eapply star_map_impl with (RA := beta) (f := fun t => switch t2 (l ++ (p2, t) :: l2)); [|assumption].
+      intros; constructor; assumption.
+Qed.
+
+
+
+Inductive pbeta : term -> term -> Prop :=
+| pbeta_var : forall n, pbeta (var n) (var n)
+| pbeta_app : forall t1 t2 t3 t4, pbeta t1 t2 -> pbeta t3 t4 -> pbeta (app t1 t3) (app t2 t4)
+| pbeta_redex : forall t1 t2 t3 t4, pbeta t1 t2 -> pbeta t3 t4 -> pbeta (app (abs t1) t3) (subst1 t4 t2)
+| pbeta_abs : forall t1 t2, pbeta t1 t2 -> pbeta (abs t1) (abs t2)
+| pbeta_constr : forall tag l1 l2, Forall2 pbeta l1 l2 -> pbeta (constr tag l1) (constr tag l2)
+| pbeta_switch : forall t1 t2 l1 l2, pbeta t1 t2 -> Forall2 (fun pt1 pt2 => fst pt1 = fst pt2 /\ pbeta (snd pt1) (snd pt2)) l1 l2 -> pbeta (switch t1 l1) (switch t2 l2)
+| pbeta_switch_redex : forall lt1 lt2 t1 t2 l1 l2,
+    Forall2 pbeta lt1 lt2 -> pbeta t1 t2 ->
+    pbeta (switch (constr (length l1) lt1) (l1 ++ (length lt1, t1) :: l2)) (subst (read_env lt2) t2).
+
+Lemma pbeta_refl :
+  forall t, pbeta t t.
+Proof.
+  induction t using term_ind2.
+  - constructor.
+  - constructor. assumption.
+  - constructor; assumption.
+  - constructor. apply Forall2_map_same. assumption.
+  - constructor; [assumption|].
+    apply Forall2_map_same. eapply Forall_impl; [|exact H].
+    intros [p t2]; simpl; tauto.
+Qed.
+
+
+Lemma Forall2_impl_transparent : forall (A B : Type) (P Q : A -> B -> Prop) (L1 : list A) (L2 : list B), (forall (x : A) (y : B), P x y -> Q x y) -> Forall2 P L1 L2 -> Forall2 Q L1 L2.
+Proof.
+  intros A B P Q L1 L2 Himpl H. induction H.
+  - constructor.
+  - constructor.
+    + apply Himpl. assumption.
+    + assumption.
+Defined.
+
+Fixpoint pbeta_ind2 (P : term -> term -> Prop)
+         (Hvar : forall n, P (var n) (var n))
+         (Happ : forall t1 t2 t3 t4, pbeta t1 t2 -> P t1 t2 -> pbeta t3 t4 -> P t3 t4 -> P (app t1 t3) (app t2 t4))
+         (Hredex : forall t1 t2 t3 t4, pbeta t1 t2 -> P t1 t2 -> pbeta t3 t4 -> P t3 t4 -> P (app (abs t1) t3) (subst1 t4 t2))
+         (Hlam : forall t1 t2, pbeta t1 t2 -> P t1 t2 -> P (abs t1) (abs t2))
+         (Hconstr : forall tag l1 l2, Forall2 pbeta l1 l2 -> Forall2 P l1 l2 -> P (constr tag l1) (constr tag l2))
+         (Hswitch : forall t1 t2 l1 l2, pbeta t1 t2 -> P t1 t2 -> Forall2 (fun pt1 pt2 => fst pt1 = fst pt2 /\ pbeta (snd pt1) (snd pt2)) l1 l2 -> Forall2 (fun pt1 pt2 => P (snd pt1) (snd pt2)) l1 l2 -> P (switch t1 l1) (switch t2 l2))
+         (Hswitch_redex : forall lt1 lt2 t1 t2 l1 l2, Forall2 pbeta lt1 lt2 -> Forall2 P lt1 lt2 -> pbeta t1 t2 -> P t1 t2 -> P (switch (constr (length l1) lt1) (l1 ++ (length lt1, t1) :: l2)) (subst (read_env lt2) t2))
+         (t1 t2 : term) (H : pbeta t1 t2) {struct H} : P t1 t2 :=
+  let rec := pbeta_ind2 P Hvar Happ Hredex Hlam Hconstr Hswitch Hswitch_redex in
+  match H with
+  | pbeta_var n => Hvar n
+  | pbeta_app t1 t2 t3 t4 H12 H34 => Happ t1 t2 t3 t4 H12 (rec t1 t2 H12) H34 (rec t3 t4 H34)
+  | pbeta_redex t1 t2 t3 t4 H12 H34 => Hredex t1 t2 t3 t4 H12 (rec t1 t2 H12) H34 (rec t3 t4 H34)
+  | pbeta_abs t1 t2 H12 => Hlam t1 t2 H12 (rec t1 t2 H12)
+  | pbeta_constr tag l1 l2 H12 =>
+    Hconstr tag l1 l2 H12
+            (Forall2_impl_transparent _ _ pbeta P l1 l2 rec H12)
+  | pbeta_switch t1 t2 l1 l2 Ht Hl =>
+    Hswitch t1 t2 l1 l2 Ht (rec t1 t2 Ht) Hl
+            (Forall2_impl_transparent _ _ _ _ l1 l2 (fun pt1 pt2 H => rec (snd pt1) (snd pt2) (match H with conj _ H2 => H2 end)) Hl)
+  | pbeta_switch_redex lt1 lt2 t1 t2 l1 l2 Hl Ht =>
+    Hswitch_redex lt1 lt2 t1 t2 l1 l2 Hl (Forall2_impl_transparent _ _ pbeta P lt1 lt2 rec Hl) Ht (rec t1 t2 Ht)
+  end.
+
+Lemma beta_pbeta :
+  forall t1 t2, beta t1 t2 -> pbeta t1 t2.
+Proof.
+  intros t1 t2 Hbeta. induction Hbeta.
+  - constructor; [assumption|apply pbeta_refl].
+  - constructor; [apply pbeta_refl|assumption].
+  - constructor; assumption.
+  - constructor; apply pbeta_refl.
+  - constructor; apply Forall2_app; [|apply Forall2_cons].
+    + apply Forall2_map_same, Forall_True; intros; apply pbeta_refl.
+    + assumption.
+    + apply Forall2_map_same, Forall_True; intros; apply pbeta_refl.
+  - constructor.
+    + assumption.
+    + apply Forall2_map_same, Forall_True; intros; split; [reflexivity|apply pbeta_refl].
+  - constructor.
+    + apply pbeta_refl.
+    + apply Forall2_app; [|apply Forall2_cons].
+      * apply Forall2_map_same, Forall_True; intros; split; [reflexivity|apply pbeta_refl].
+      * split; [reflexivity|assumption].
+      * apply Forall2_map_same, Forall_True; intros; split; [reflexivity|apply pbeta_refl].
+  - constructor; [|apply pbeta_refl].
+    apply Forall2_map_same, Forall_True; intros; apply pbeta_refl.
+Qed.
+
+Lemma Forall2_and :
+  forall (A B : Type) (P Q : A -> B -> Prop) L1 L2, Forall2 P L1 L2 -> Forall2 Q L1 L2 -> Forall2 (fun x y => P x y /\ Q x y) L1 L2.
+Proof.
+  intros A B P Q L1 L2 HP. induction HP; intros HQ; inversion HQ; subst.
+  - constructor.
+  - constructor; [split; assumption|apply IHHP; assumption].
+Qed.
+
+Lemma Forall2_length :
+  forall (A B : Type) (P : A -> B -> Prop) L1 L2, Forall2 P L1 L2 -> length L1 = length L2.
+Proof.
+  intros A B P L1 L2 H. induction H; simpl; congruence.
+Qed.
+
+Lemma pbeta_star_beta :
+  forall t1 t2, pbeta t1 t2 -> star beta t1 t2.
+Proof.
+  intros t1 t2 Hpbeta. induction Hpbeta using pbeta_ind2.
+  - constructor.
+  - apply star_beta_app; assumption.
+  - eapply star_compose.
+    + apply star_beta_app; [|eassumption].
+      apply star_beta_abs; eassumption.
+    + econstructor; [|constructor]. constructor.
+  - eapply star_map_impl with (RA := beta) (f := abs); [|assumption].
+    intros; constructor; assumption.
+  - apply star_beta_constr; assumption.
+  - apply star_beta_switch; [assumption|].
+    eapply Forall2_impl; [|apply Forall2_and; [apply H|apply H0]].
+    intros; simpl in *; tauto.
+  - eapply star_compose; [|eapply star_compose].
+    + eapply star_map_impl with (RA := beta) (f := fun t => switch t _); [intros; constructor; assumption|].
+      apply star_beta_constr. eassumption.
+    + eapply star_map_impl with (RA := beta) (f := fun t => switch _ (_ ++ (_, t) :: _)); [|eassumption].
+      intros; simpl; constructor; assumption.
+    + econstructor; [|constructor].
+      rewrite (Forall2_length _ _ _ _ _ H).
+      constructor.
+Qed.
+
+Lemma nth_error_Forall2_iff:
+  forall A B (P : A -> B -> Prop) L1 L2,
+    Forall2 P L1 L2 <-> (length L1 = length L2 /\ forall n x y, nth_error L1 n = Some x -> nth_error L2 n = Some y -> P x y).
+Proof.
+  intros A B P L1 L2. split.
+  - intros H. induction H.
+    + split; [reflexivity|]. intros; destruct n; simpl in *; discriminate.
+    + destruct IHForall2 as [Hlen Hforall].
+      split; [simpl; congruence|].
+      intros [|n]; simpl; [|apply Hforall].
+      intros; congruence.
+  - revert L2; induction L1 as [|x L1 IH]; intros [|y L2] [Hlen Hforall]; simpl in *.
+    + constructor.
+    + discriminate.
+    + discriminate.
+    + constructor; [apply (Hforall 0); reflexivity|].
+      apply IH. split; [congruence|].
+      intros n; apply (Hforall (S n)).
+Qed.
+
+Lemma nth_error_Forall_iff :
+  forall A (P : A -> Prop) L,
+    Forall P L <-> (forall n x, nth_error L n = Some x -> P x).
+Proof.
+  intros A P L. split.
+  - intros H. induction H.
+    + intros; destruct n; simpl in *; discriminate.
+    + intros [|n]; simpl; [|apply IHForall].
+      intros; congruence.
+  - induction L as [|x L IH]; intros Hforall; simpl in *.
+    + constructor.
+    + constructor.
+      * apply (Hforall 0); reflexivity.
+      * apply IH. intros n; apply (Hforall (S n)).
+Qed.
+
+Ltac ereplace t :=
+  let tmp := fresh "_tmp" in
+  let typ := type of t in
+  evar (tmp : typ);
+  replace t with tmp; unfold tmp.
+
+
+Lemma subst_subst1 :
+  forall us t1 t2, subst us (subst1 t1 t2) = subst1 (subst us t1) (subst (lift_subst us) t2).
+Proof.
+  intros us t1 t2. unfold subst1. rewrite !subst_subst.
+  apply subst_ext. unfold comp. intros [|n].
+  * reflexivity.
+  * simpl. unfold comp. rewrite subst_ren.
+    etransitivity; [symmetry; apply subst_id|].
+    apply subst_ext. intros n1. unfold comp. simpl. f_equal. lia.
+Qed.
+
+Lemma lift_ren :
+  forall r n, ren (lift r) n = lift_subst (ren r) n.
+Proof.
+  intros r n. unfold ren, lift_subst, comp.
+  rewrite lift_renv. simpl.
+  destruct n; simpl; [reflexivity|].
+  f_equal; lia.
+Qed.
+
+Lemma ren_subst1 :
+  forall r t1 t2, ren_term r (subst1 t1 t2) = subst1 (ren_term r t1) (ren_term (lift r) t2).
+Proof.
+  intros r t1 t2.
+  rewrite !ren_term_is_subst, subst_subst1.
+  f_equal. apply subst_ext.
+  intros n; rewrite lift_ren; reflexivity.
+Qed.
+
+Lemma subst_read_env :
+  forall us l t, subst us (subst (read_env l) t) = subst (read_env (map (subst us) l)) (subst (liftn_subst (length l) us) t).
+Proof.
+  intros us l t. rewrite !subst_subst. apply subst_ext; intros n.
+  unfold comp, read_env, liftn_subst.
+  destruct nth_error as [u|] eqn:Hln.
+  - destruct le_lt_dec; [apply nth_error_None in l0; congruence|]. simpl.
+    rewrite nth_error_map, Hln. reflexivity.
+  - destruct le_lt_dec; [|apply nth_error_None in Hln; lia].
+    simpl. rewrite subst_ren.
+    etransitivity; [symmetry; apply subst_id|].
+    eapply subst_ext.
+    intros m. unfold comp, ren. simpl.
+    rewrite plus_ren_correct.
+    replace (nth_error _ _) with (@None term).
+    + f_equal. rewrite map_length. lia.
+    + symmetry. apply nth_error_None. rewrite map_length; lia.
+Qed.
+
+Lemma ren_read_env :
+  forall r l t, ren_term r (subst (read_env l) t) = subst (read_env (map (ren_term r) l)) (ren_term (liftn (length l) r) t).
+Proof.
+  intros r l t.
+  rewrite !ren_term_is_subst, subst_read_env.
+  f_equal.
+  - f_equal. apply map_ext. intros; rewrite ren_term_is_subst; reflexivity.
+  - apply subst_ext. intros n.
+    unfold liftn_subst, ren. destruct le_lt_dec; simpl.
+    + rewrite plus_ren_correct.
+      rewrite liftn_renv_large; [reflexivity|assumption].
+    + rewrite liftn_renv_small; [reflexivity|assumption].
+Qed.
+
+Lemma pbeta_ren : forall t1 t2 r, pbeta t1 t2 -> pbeta (ren_term r t1) (ren_term r t2).
+Proof.
+  intros t1 t2 r H. revert r. induction H using pbeta_ind2; intros r; simpl in *.
+  - constructor.
+  - constructor; [apply IHpbeta1|apply IHpbeta2].
+  - rewrite ren_subst1.
+    constructor; [apply IHpbeta1|apply IHpbeta2].
+  - constructor; apply IHpbeta.
+  - constructor. apply Forall2_map_left, Forall2_map_right.
+    eapply Forall2_impl; [|eassumption]. intros; auto.
+  - constructor; [apply IHpbeta|].
+    apply Forall2_map_left, Forall2_map_right.
+    eapply Forall2_impl; [|apply Forall2_and; [apply H0|apply H1]].
+    simpl.
+    intros [p3 t3] [p4 t4] [[Heq Hbeta] IH].
+    split; [assumption|]. simpl in *. subst.
+    apply IH.
+  - rewrite map_app. simpl.
+    ereplace (length l1); [|eapply map_length].
+    ereplace (length lt1); [|eapply map_length].
+    rewrite ren_read_env.
+    constructor.
+    + rewrite Forall2_map_left, Forall2_map_right.
+      eapply Forall2_impl; [|exact H0].
+      simpl. intros; auto.
+    + rewrite map_length, (Forall2_length _ _ _ _ _ H).
+      apply IHpbeta.
+Qed.
+
+Lemma pbeta_subst : forall t1 t2 us1 us2, pbeta t1 t2 -> (forall n, pbeta (us1 n) (us2 n)) -> pbeta (subst us1 t1) (subst us2 t2).
+Proof.
+  intros t1 t2 us1 us2 H. revert us1 us2. induction H using pbeta_ind2; intros us1 us2 Hus; simpl in *.
+  - apply Hus.
+  - constructor; [apply IHpbeta1|apply IHpbeta2]; assumption.
+  - rewrite subst_subst1.
+    constructor; [apply IHpbeta1|apply IHpbeta2; assumption].
+    intros [|n]; simpl; [constructor|].
+    unfold comp. apply pbeta_ren, Hus.
+  - constructor. apply IHpbeta.
+    intros [|n]; simpl; [constructor|].
+    unfold comp. apply pbeta_ren, Hus.
+  - constructor. apply Forall2_map_left, Forall2_map_right.
+    eapply Forall2_impl; [|eassumption].
+    intros; simpl in *; auto.
+  - constructor.
+    + apply IHpbeta. assumption.
+    + rewrite Forall2_map_left, Forall2_map_right. simpl.
+      eapply Forall2_impl; [|apply Forall2_and; [apply H0|apply H1]].
+      simpl.
+      intros [p3 t3] [p4 t4] [[Heq Hbeta] IH].
+      split; [assumption|]. simpl in *. subst.
+      apply IH.
+      intros n. unfold liftn_subst.
+      destruct le_lt_dec; [apply pbeta_ren; apply Hus|apply pbeta_refl].
+  - rewrite map_app. simpl.
+    ereplace (length l1); [|eapply map_length].
+    ereplace (length lt1); [|eapply map_length].
+    rewrite subst_read_env.
+    constructor.
+    + rewrite Forall2_map_left, Forall2_map_right.
+      eapply Forall2_impl; [|exact H0].
+      simpl. intros; auto.
+    + rewrite map_length, (Forall2_length _ _ _ _ _ H).
+      apply IHpbeta.
+      intros n; unfold liftn_subst. destruct le_lt_dec; [apply pbeta_ren; apply Hus|apply pbeta_refl].
+Qed.
+
+Lemma read_env_pbeta :
+  forall l1 l2, Forall2 pbeta l1 l2 -> forall n, pbeta (read_env l1 n) (read_env l2 n).
+Proof.
+  intros l1 l2 H n. unfold read_env.
+  destruct (nth_error l1 n) eqn:H1.
+  - destruct (nth_error l2 n) eqn:H2.
+    + rewrite nth_error_Forall2_iff in H; eapply H; eassumption.
+    + erewrite nth_error_Forall2_None in H2; [|eapply Forall2_comm; exact H]. congruence.
+  - erewrite nth_error_Forall2_None in H1; [|exact H].
+    rewrite H1. rewrite nth_error_Forall2_iff in H; rewrite (proj1 H).
+    apply pbeta_refl.
+Qed.
+
+Lemma list_exists :
+  forall (A : Type) (P : nat -> A -> Prop) n, (forall k, k < n -> exists x, P k x) -> exists L, length L = n /\ (forall k x, nth_error L k = Some x -> P k x).
+Proof.
+  intros A P n. induction n; intros H.
+  - exists nil. split; [reflexivity|].
+    intros [|k]; simpl; intros; discriminate.
+  - destruct IHn as [L HL]; [intros k Hk; apply H; lia|].
+    destruct (H n) as [x Hx]; [lia|].
+    exists (L ++ x :: nil). split.
+    + rewrite app_length; simpl. lia.
+    + intros k y.
+      destruct (le_lt_dec n k).
+      * rewrite nth_error_app2 by lia.
+        destruct (k - length L) as [|u] eqn:Hu; simpl.
+        -- assert (k = n) by lia. congruence.
+        -- destruct u; simpl; discriminate.
+      * rewrite nth_error_app1 by lia. apply HL.
+Qed.
+
+Lemma nth_error_Some2 :
+  forall (A : Type) (l : list A) n, n < length l -> exists x, nth_error l n = Some x.
+Proof.
+  intros A l n. revert l; induction n; intros l H; destruct l as [|x l]; simpl in *; try lia.
+  - exists x. reflexivity.
+  - apply IHn. lia.
+Qed.
+
+Lemma nth_error_Some3 :
+  forall (A : Type) (l : list A) n x, nth_error l n = Some x -> n < length l.
+Proof.
+  intros. apply nth_error_Some. destruct nth_error; congruence.
+Qed.
+
+
+Inductive Forall3 {A B C : Type} (R : A -> B -> C -> Prop) : list A -> list B -> list C -> Prop :=
+| Forall3_nil : Forall3 R nil nil nil
+| Forall3_cons : forall x y z l1 l2 l3, R x y z -> Forall3 R l1 l2 l3 -> Forall3 R (x :: l1) (y :: l2) (z :: l3).
+
+Inductive Forall4 {A B C D : Type} (R : A -> B -> C -> D -> Prop) : list A -> list B -> list C -> list D -> Prop :=
+| Forall4_nil : Forall4 R nil nil nil nil
+| Forall4_cons : forall x y z w l1 l2 l3 l4, R x y z w -> Forall4 R l1 l2 l3 l4 -> Forall4 R (x :: l1) (y :: l2) (z :: l3) (w :: l4).
+
+Lemma Forall3_select12 :
+  forall A B C R (l1 : list A) (l2 : list B) (l3 : list C),
+    Forall3 (fun x y z => R x y) l1 l2 l3 -> Forall2 R l1 l2.
+Proof.
+  intros A B C R l1 l2 l3 H; induction H; constructor; auto.
+Qed.
+
+Lemma Forall3_select13 :
+  forall A B C R (l1 : list A) (l2 : list B) (l3 : list C),
+    Forall3 (fun x y z => R x z) l1 l2 l3 -> Forall2 R l1 l3.
+Proof.
+  intros A B C R l1 l2 l3 H; induction H; constructor; auto.
+Qed.
+
+Lemma Forall3_select23 :
+  forall A B C R (l1 : list A) (l2 : list B) (l3 : list C),
+    Forall3 (fun x y z => R y z) l1 l2 l3 -> Forall2 R l2 l3.
+Proof.
+  intros A B C R l1 l2 l3 H; induction H; constructor; auto.
+Qed.
+
+Lemma Forall4_select123 :
+  forall A B C D R (l1 : list A) (l2 : list B) (l3 : list C) (l4 : list D),
+    Forall4 (fun x y z w => R x y z) l1 l2 l3 l4 -> Forall3 R l1 l2 l3.
+Proof.
+  intros A B C D R l1 l2 l3 l4 H; induction H; constructor; auto.
+Qed.
+
+Lemma Forall4_select124 :
+  forall A B C D R (l1 : list A) (l2 : list B) (l3 : list C) (l4 : list D),
+    Forall4 (fun x y z w => R x y w) l1 l2 l3 l4 -> Forall3 R l1 l2 l4.
+Proof.
+  intros A B C D R l1 l2 l3 l4 H; induction H; constructor; auto.
+Qed.
+
+Lemma Forall4_select134 :
+  forall A B C D R (l1 : list A) (l2 : list B) (l3 : list C) (l4 : list D),
+    Forall4 (fun x y z w => R x z w) l1 l2 l3 l4 -> Forall3 R l1 l3 l4.
+Proof.
+  intros A B C D R l1 l2 l3 l4 H; induction H; constructor; auto.
+Qed.
+
+Lemma Forall4_select234 :
+  forall A B C D R (l1 : list A) (l2 : list B) (l3 : list C) (l4 : list D),
+    Forall4 (fun x y z w => R y z w) l1 l2 l3 l4 -> Forall3 R l2 l3 l4.
+Proof.
+  intros A B C D R l1 l2 l3 l4 H; induction H; constructor; auto.
+Qed.
+
+Lemma Forall4_select12 :
+  forall A B C D R (l1 : list A) (l2 : list B) (l3 : list C) (l4 : list D),
+    Forall4 (fun x y z w => R x y) l1 l2 l3 l4 -> Forall2 R l1 l2.
+Proof.
+  intros A B C D R l1 l2 l3 l4 H; induction H; constructor; auto.
+Qed.
+
+Lemma Forall4_select13 :
+  forall A B C D R (l1 : list A) (l2 : list B) (l3 : list C) (l4 : list D),
+    Forall4 (fun x y z w => R x z) l1 l2 l3 l4 -> Forall2 R l1 l3.
+Proof.
+  intros A B C D R l1 l2 l3 l4 H; induction H; constructor; auto.
+Qed.
+
+Lemma Forall4_select14 :
+  forall A B C D R (l1 : list A) (l2 : list B) (l3 : list C) (l4 : list D),
+    Forall4 (fun x y z w => R x w) l1 l2 l3 l4 -> Forall2 R l1 l4.
+Proof.
+  intros A B C D R l1 l2 l3 l4 H; induction H; constructor; auto.
+Qed.
+
+Lemma Forall4_select23 :
+  forall A B C D R (l1 : list A) (l2 : list B) (l3 : list C) (l4 : list D),
+    Forall4 (fun x y z w => R y z) l1 l2 l3 l4 -> Forall2 R l2 l3.
+Proof.
+  intros A B C D R l1 l2 l3 l4 H; induction H; constructor; auto.
+Qed.
+
+Lemma Forall4_select24 :
+  forall A B C D R (l1 : list A) (l2 : list B) (l3 : list C) (l4 : list D),
+    Forall4 (fun x y z w => R y w) l1 l2 l3 l4 -> Forall2 R l2 l4.
+Proof.
+  intros A B C D R l1 l2 l3 l4 H; induction H; constructor; auto.
+Qed.
+
+Lemma Forall4_select34 :
+  forall A B C D R (l1 : list A) (l2 : list B) (l3 : list C) (l4 : list D),
+    Forall4 (fun x y z w => R z w) l1 l2 l3 l4 -> Forall2 R l3 l4.
+Proof.
+  intros A B C D R l1 l2 l3 l4 H; induction H; constructor; auto.
+Qed.
+
+
+
+Lemma Forall_exists_Forall2 :
+  forall (A B : Type) (P : A -> B -> Prop) (l1 : list A),
+    Forall (fun x => exists y, P x y) l1 -> exists l2, Forall2 P l1 l2.
+Proof.
+  intros A B P l1 H; induction H.
+  - exists nil. constructor.
+  - destruct IHForall as [l2 IH].
+    destruct H as [y Hy].
+    exists (y :: l2). constructor; assumption.
+Qed.
+
+Lemma Forall2_exists_Forall3 :
+  forall (A B C : Type) (P : A -> B -> C -> Prop) (l1 : list A) (l2 : list B),
+    Forall2 (fun x y => exists z, P x y z) l1 l2 -> exists l3, Forall3 P l1 l2 l3.
+Proof.
+  intros A B C P l1 l2 H; induction H.
+  - exists nil. constructor.
+  - destruct IHForall2 as [l3 IH].
+    destruct H as [z Hz].
+    exists (z :: l3). constructor; assumption.
+Qed.
+
+Lemma Forall3_exists_Forall4 :
+  forall (A B C D: Type) (P : A -> B -> C -> D -> Prop) (l1 : list A) (l2 : list B) (l3 : list C),
+    Forall3 (fun x y z => exists w, P x y z w) l1 l2 l3 -> exists l4, Forall4 P l1 l2 l3 l4.
+Proof.
+  intros A B C D P l1 l2 l3 H; induction H.
+  - exists nil. constructor.
+  - destruct IHForall3 as [l4 IH].
+    destruct H as [w Hw].
+    exists (w :: l4). constructor; assumption.
+Qed.
+
+
+Lemma Forall3_impl :
+  forall (A B C : Type) (P Q : A -> B -> C -> Prop) l1 l2 l3,
+    (forall x y z, P x y z -> Q x y z) -> Forall3 P l1 l2 l3 -> Forall3 Q l1 l2 l3.
+Proof.
+  intros A B C P Q l1 l2 l3 HPQ H; induction H; constructor; [apply HPQ|]; assumption.
+Qed.
+
+Lemma Forall4_impl :
+  forall (A B C D : Type) (P Q : A -> B -> C -> D -> Prop) l1 l2 l3 l4,
+    (forall x y z w, P x y z w -> Q x y z w) -> Forall4 P l1 l2 l3 l4 -> Forall4 Q l1 l2 l3 l4.
+Proof.
+  intros A B C D P Q l1 l2 l3 l4 HPQ H; induction H; constructor; [apply HPQ|]; assumption.
+Qed.
+
+
+Lemma Forall3_from_Forall2 :
+  forall (A B C : Type) (P : A -> B -> Prop) (Q : A -> C -> Prop) l1 l2 l3,
+    Forall2 P l1 l2 -> Forall2 Q l1 l3 -> Forall3 (fun x y z => P x y /\ Q x z) l1 l2 l3.
+Proof.
+  intros A B C P Q l1 l2 l3 H1. revert l3; induction H1; intros l3 H2; inversion H2; subst.
+  - constructor.
+  - constructor.
+    + split; assumption.
+    + apply IHForall2. assumption.
+Qed.
+
+Lemma list_app_eq_length :
+  forall A (l1 l2 l3 l4 : list A), l1 ++ l3 = l2 ++ l4 -> length l1 = length l2 -> l1 = l2 /\ l3 = l4.
+Proof.
+  intros A l1 l2 l3 l4; revert l2; induction l1; intros l2 H1 H2; destruct l2; simpl in *; try intuition congruence.
+  specialize (IHl1 l2 ltac:(congruence) ltac:(congruence)).
+  intuition congruence.
+Qed.
+
+
+Definition locally_confluent {A : Type} (R : A -> A -> Prop) :=
+  forall x y z, R x y -> R x z -> exists w, R y w /\ R z w.
+
+Definition confluent {A : Type} (R : A -> A -> Prop) := locally_confluent (star R).
+
+Lemma pbeta_lc : locally_confluent pbeta.
+Proof.
+  intros t1 t2 t3 H12. revert t3. induction H12 using pbeta_ind2; intros t5 H15; inversion H15; subst.
+  - exists (var n). split; constructor.
+  - destruct (IHpbeta1 t6) as (t7 & H27 & H67); [assumption|].
+    destruct (IHpbeta2 t8) as (t9 & H49 & H89); [assumption|].
+    exists (app t7 t9). split; constructor; assumption.
+  - destruct (IHpbeta1 (abs t6)) as (t7 & H27 & H67); [constructor; assumption|].
+    destruct (IHpbeta2 t8) as (t9 & H49 & H89); [assumption|].
+    inversion H67; subst.
+    inversion H12_; subst.
+    exists (subst1 t9 t5). split.
+    + constructor; [inversion H27; subst; assumption|assumption].
+    + apply pbeta_subst; [assumption|].
+      intros [|n]; simpl; [assumption|constructor].
+  - inversion H1; subst.
+    destruct (IHpbeta1 t5) as (t7 & H27 & H57); [assumption|].
+    destruct (IHpbeta2 t8) as (t9 & H49 & H89); [assumption|].
+    exists (subst1 t9 t7). split.
+    + apply pbeta_subst; [assumption|].
+      intros [|n]; simpl; [assumption|constructor].
+    + constructor; assumption.
+  - destruct (IHpbeta1 t6) as (t7 & H27 & H67); [assumption|].
+    destruct (IHpbeta2 t8) as (t9 & H49 & H89); [assumption|].
+    exists (subst1 t9 t7). split; apply pbeta_subst.
+    + assumption.
+    + intros [|n]; simpl; [assumption|constructor].
+    + assumption.
+    + intros [|n]; simpl; [assumption|constructor].
+  - destruct (IHpbeta t3) as (t4 & H24 & H34); [assumption|].
+    exists (abs t4); split; constructor; assumption.
+  - assert (H23 := Forall3_from_Forall2 _ _ _ _ _ _ _ _ H0 H4).
+    simpl in *.
+    eapply Forall3_impl in H23; [|intros x y z H123; exact (proj1 H123 z (proj2 H123))].
+    apply Forall3_select23 in H23.
+    apply Forall2_exists_Forall3 in H23.
+    destruct H23 as (l4 & Hl4).
+    exists (constr tag l4).
+    split; constructor.
+    + eapply Forall3_select13; eapply Forall3_impl; [|apply Hl4]. intros; simpl in *; tauto.
+    + eapply Forall3_select23; eapply Forall3_impl; [|apply Hl4]. intros; simpl in *; tauto.
+  - assert (H23 := Forall3_from_Forall2 _ _ _ _ _ _ _ _ (Forall2_and _ _ _ _ _ _ H H0) H5).
+    simpl in *.
+    eapply Forall3_impl in H23.
+    + eapply Forall3_select23 in H23. eapply Forall2_exists_Forall3 in H23. destruct H23 as (l4 & Hl4).
+      destruct (IHpbeta _ H3) as (t4 & Ht4).
+      exists (switch t4 l4).
+      split; constructor.
+      * tauto.
+      * eapply Forall3_select13; eapply Forall3_impl; [|apply Hl4]. intros x y z Hxyz; refine (proj1 Hxyz). shelve.
+      * tauto.
+      * eapply Forall3_select23; eapply Forall3_impl; [|apply Hl4]. intros x y z Hxyz; exact (proj2 Hxyz).
+    + simpl. intros x y z (((Ha & Hb) & Hc) & Hd & He).
+      destruct (Hc _ He) as (t4 & Ht4). exists (fst z, t4). simpl.
+      intuition congruence.
+  - assert (H6 := Forall2_and _ _ _ _ _ _ H0 H). simpl in *.
+    apply Forall2_app_inv_l in H6. destruct H6 as (l2a & l2b & H6a & H6b & H6eq).
+    inversion H6b; subst; simpl in *.
+    destruct y as [p t1]; destruct H4 as [H4 [Hp Ht1]]; simpl in *; subst.
+    destruct (H4 _ H5) as (t4 & Ht4).
+    inversion H12; subst.
+    destruct (IHpbeta (constr (length l0) lt2) ltac:(constructor; assumption)) as (t5 & Ht5a & Ht5b).
+    inversion Ht5a; subst. inversion Ht5b; subst.
+    exists (subst (read_env l4) t4).
+    split.
+    + rewrite (Forall2_length _ _ _ _ _ H6a).
+      rewrite (Forall2_length _ _ _ _ _ H8).
+      constructor; tauto.
+    + apply pbeta_subst; [tauto|].
+      apply read_env_pbeta. assumption.
+  - apply Forall2_app_inv_l in H5. destruct H5 as (l2a & l2b & H5a & H5b & H5eq).
+    inversion H5b; subst; simpl in *.
+    destruct y as [p t4]; destruct H4 as [Hp Ht4]; simpl in *; subst.
+    destruct (IHpbeta _ Ht4) as (t5 & Ht5).
+    inversion H3; subst.
+    assert (H7 := Forall3_from_Forall2 _ _ _ _ _ _ _ _ H0 H5).
+    simpl in *.
+    eapply Forall3_impl in H7; [|intros x y z Hxyz; exact (proj1 Hxyz z (proj2 Hxyz))].
+    apply Forall3_select23, Forall2_exists_Forall3 in H7.
+    destruct H7 as (l4 & Hl4).
+    exists (subst (read_env l4) t5).
+    split.
+    + apply pbeta_subst; [tauto|].
+      apply read_env_pbeta. eapply Forall3_select13, Forall3_impl, Hl4. intros; simpl in *; tauto.
+    + rewrite (Forall2_length _ _ _ _ _ H5a).
+      rewrite (Forall2_length _ _ _ _ _ H5).
+      constructor; [|tauto]. eapply Forall3_select23, Forall3_impl, Hl4. intros; simpl in *; tauto.
+  - apply list_app_eq_length in H4; [|assumption].
+    destruct H4 as (? & [=]); subst.
+    destruct (IHpbeta _ H6) as (t4 & Ht4).
+    assert (H23 := Forall3_from_Forall2 _ _ _ _ _ _ _ _ H0 H5).
+    simpl in *.
+    eapply Forall3_impl in H23; [|intros x y z H123; exact (proj1 H123 z (proj2 H123))].
+    apply Forall3_select23 in H23.
+    apply Forall2_exists_Forall3 in H23.
+    destruct H23 as (lt4 & Hlt4).
+    exists (subst (read_env lt4) t4).
+    split; eapply pbeta_subst; try apply Ht4; apply read_env_pbeta.
+    + eapply Forall3_select13, Forall3_impl, Hlt4; intros; simpl in *; tauto.
+    + eapply Forall3_select23, Forall3_impl, Hlt4; intros; simpl in *; tauto.
+Qed.
+
+Lemma lc_is_confluent :
+  forall (A : Type) (R : A -> A -> Prop), locally_confluent R -> confluent R.
+Proof.
+  intros A R H.
+  assert (H1 : forall x y z, star R x y -> R x z -> exists w, star R z w /\ R y w).
+  - intros x y z Hxy; revert z. induction Hxy.
+    + intros z Hxz. exists z. split; [apply star_refl|assumption].
+    + intros w Hw. destruct (H _ _ _ H0 Hw) as (t & Hyt & Hwt).
+      destruct (IHHxy t Hyt) as (s & Hs1 & Hs2).
+      exists s. split; [|assumption]. econstructor; eassumption.
+  - intros x y z Hxy; revert z. induction Hxy.
+    + intros z Hxz; exists z. split; [assumption|apply star_refl].
+    + intros w Hxw. destruct (H1 _ _ _ Hxw H0) as (t & Ht1 & Ht2).
+      destruct (IHHxy _ Ht1) as (s & Hs1 & Hs2).
+      exists s. split; [assumption|]. econstructor; eassumption.
+Qed.
+
+Lemma star_beta_is_star_pbeta :
+  forall x y, star beta x y <-> star pbeta x y.
+Proof.
+  intros x y. split; intros H.
+  - eapply star_map_impl with (f := id); [|eassumption].
+    intros x1 y1; simpl. apply beta_pbeta.
+  - eapply star_star.
+    eapply star_map_impl with (f := id); [|eassumption].
+    intros x1 y1; simpl. apply pbeta_star_beta.
+Qed.
+
+Lemma locally_confluent_ext :
+  forall (A : Type) (R1 R2 : A -> A -> Prop), (forall x y, R1 x y <-> R2 x y) -> locally_confluent R1 <-> locally_confluent R2.
+Proof.
+  intros A R1 R2 Heq; split; intros H x y z Hxy Hxz.
+  - rewrite <- Heq in Hxy, Hxz. destruct (H _ _ _ Hxy Hxz) as (w & Hyw & Hzw).
+    exists w; split; rewrite <- Heq; assumption.
+  - rewrite Heq in Hxy, Hxz. destruct (H _ _ _ Hxy Hxz) as (w & Hyw & Hzw).
+    exists w; split; rewrite Heq; assumption.
+Qed.
+
+Lemma beta_confluent :
+  confluent beta.
+Proof.
+  eapply locally_confluent_ext; [apply star_beta_is_star_pbeta|].
+  apply lc_is_confluent, pbeta_lc.
+Qed.
